Nicer notation

ModalTypes/WellTyped.lean
@@ -3,7 +3,7 @@ import ModalTypes.Type
 import ModalTypes.Context
 import Aesop
 
-open Ty
+open Ty 
 
 @[aesop safe constructors]
 inductive WellTyped : Context → Term → Ty → Prop
@@ -13,29 +13,30 @@ inductive WellTyped : Context → Term → Ty → Prop
   -/
   | var : Γ.get? x = some A → WellTyped (Γ::Γs) (.var x) A
   /-- Standard rule for lambdas -/
-  | lam : WellTyped (Γ.add A) t B → WellTyped Γ (.lam A t) [| A → B |]
+  | lam : WellTyped (Γ.add A) t B → WellTyped Γ (.lam A t) ⟪ A → B ⟫
   /-- Standard rule for application -/
-  | app (A) : WellTyped Γ f [| A → B|] → WellTyped Γ t A → WellTyped Γ (.app f t) B
+  | app (A) : WellTyped Γ f ⟪ A → B⟫ → WellTyped Γ t A → WellTyped Γ (.app f t) B
   /-- Standard rule for products -/
-  | prod : WellTyped Γ t A → WellTyped Γ u B → WellTyped Γ (.pair t u) [| A × B |]
+  | prod : WellTyped Γ t A → WellTyped Γ u B → WellTyped Γ (.pair t u) ⟪ A × B ⟫
   /-- Standard rule for sums -/
-  | inl : WellTyped Γ t A → WellTyped Γ (.inl t) [| A + B |]
+  | inl : WellTyped Γ t A → WellTyped Γ (.inl t) ⟪ A + B ⟫
   /-- Standard rule for sums -/
-  | inr : WellTyped Γ t B → WellTyped Γ (.inr t) [| A + B |]
-  | fst : WellTyped Γ t [| A × B |] → WellTyped Γ (.fst t) A
-  | snd : WellTyped Γ t [| A × B |] → WellTyped Γ (.snd t) B
+  | inr : WellTyped Γ t B → WellTyped Γ (.inr t) ⟪ A + B ⟫
+  | fst : WellTyped Γ t ⟪ A × B ⟫ → WellTyped Γ (.fst t) A
+  | snd : WellTyped Γ t ⟪ A × B ⟫ → WellTyped Γ (.snd t) B
   /-
     TODO: in this encoding of the shut rule, `Γ'` cannot contain any more locks, but the original
       has no such restriction.
       We could turn this into `Γ' ++ Γ` with the restriction that `Γ' ≠ []`, or
-        `Γs ++ (Γ'::Γ)` without such an extra assumption (I choose this second option for now)
+        `Γs ++ (Γ'::Γ)` without such an extra assumption 
+      (I choose this second option for now)
   -/
-  | open : WellTyped Γ t [| □A |] → WellTyped (Γs ++ Γ'::Γ) (.open t) A
-  | shut : WellTyped ([]::Γ) t A → WellTyped Γ (.shut t) [| □A |]
+  | open : WellTyped Γ t ⟪ □A ⟫ → WellTyped (Γs ++ Γ'::Γ) (.open t) A
+  | shut : WellTyped ([]::Γ) t A → WellTyped Γ (.shut t) ⟪ □A ⟫
 
 
 
-example : ∃ t, WellTyped [] t [| □(A → B) → □A → □B |] := by
+example : ∃ t, WellTyped [] t ⟪ □(A → B) → □A → □B ⟫ := by
   refine ⟨
     .lam _ <| .lam _ <| .shut <| .app (.open <| .var 1) (.open <| .var 0),
     .lam <| .lam <| .shut ?h
